\small
$$
X =
\begin{bmatrix}
1 & \cdot \\[-.2em]
\cdot & 1
\end{bmatrix}\!\!,
Y =
\begin{bmatrix}
1
\end{bmatrix}\!\!,
$$
$$
\bar{X} = X\oplus (1,0) =
\begin{bmatrix}
\cdot & \cdot \\[-.2em]
1 & \cdot \\[-.2em]
\cdot & 1
\end{bmatrix}\!\!,
$$
$$
\bar{Y} = Y\oplus (1,1) =
\begin{bmatrix}
\cdot & \cdot \\[-.2em]
\cdot & 1 \\[-.2em]
\cdot & \cdot
\end{bmatrix}\!\!,
$$
$$
\bar{X} + \bar{Y} =
\begin{bmatrix}
\cdot & \cdot \\[-.2em]
1 & 1 \\[-.2em]
\cdot & 1
\end{bmatrix}\!\!,
$$
$$
Z = \ominus(\bar{X}+\bar{Y})=
\begin{bmatrix}
1 & 1 \\[-.2em]
\cdot & 1
\end{bmatrix}\!\!
$$
\caption{Example of Theorem \ref{fundamental}. The $2\times 3$ input matrix is not shown.}